# Calculus

## Diagnostic Test

**1.**

> Evaluate each expression without using a calculator.

- $ (-3)^4 $

$$
  (-3)^4 = 3^4 = 81
$$

- $ -3^4 $

$$
  -3^4 = -(3^4) = -81
$$

- $ 3^{-4} $

$$
  3^{-4} = \dfrac{1}{3^4} = \dfrac{1}{81}
$$

- $ \dfrac{ 5^{23} }{ 5^{21} } $

$$
  \dfrac{ 5^{23} }{ 5^{21} } = 5^{23-21} = 5^2 = 25
$$

- $ \left( \dfrac{2}{3} \right) ^{-2} $

$$
  \left( \dfrac{2}{3} \right) ^{-2} = \left( \dfrac{3}{2} \right) ^2 = \dfrac{9}{4}
$$

- $ 16^{-3/4} $

$$
  16^{-3/4} = \dfrac{1}{16^{3/4}} = \dfrac{1}{\sqrt[4]{16}^3} = \dfrac{1}{2^3} = \dfrac{1}{8}
$$

**2.**
> Simplify each expression. Write your answer without negative exponents.

- $ \sqrt{200} - \sqrt{32} $

$$
  \sqrt{200} - \sqrt{32} = \sqrt{100 \cdot 2} - \sqrt{16 \cdot 2} = 10\sqrt{2} - 4\sqrt{2} = 6\sqrt{2}
$$

- $ (3 a^3 b^3) (4 a b^2)^2 $

$$
(3 a^3 b^3) (4 a b^2)^2 = (3 a^3 b^3) (16 a^2 b^4) = 48 a^5 b^7
$$

- $ \left( \dfrac{ 3 x^{3/2} y^3 }{ x^2 y^{-1/2} } \right) ^{-2} $

$$
  \left( \dfrac{ 3 x^{3/2} y^3 }{ x^2 y^{-1/2} } \right) ^{-2}
= \left( \dfrac{ x^2 y^{-1/2} }{ 3 x^{3/2} y^3 } \right) ^2
= \left( \dfrac{ x^4 y^{-1} }{ 9 x^{3} y^6 } \right)
= \dfrac{1}{9} x y^{-7} = \dfrac{x}{9 y^7}  
$$

**3.**
> Expand and simplify.

- $ 3(x + 6) + 4(2x - 5) $

$$
  3(x + 6) + 4(2x - 5) = 3x + 18 + 8x - 20 = 11x - 2
$$

- $ (x + 3)(4x - 5) $

$$
  (x + 3)(4x - 5) = 4x^2 - 5x + 12x - 15 = 4x^2 + 7x - 15
$$

- $ (\sqrt{a} + \sqrt{b})(\sqrt{a} - \sqrt{b}) $

$$
  (\sqrt{a} + \sqrt{b})(\sqrt{a} - \sqrt{b}) = (\sqrt{a})^2 - (\sqrt{b})^2 = a - b
$$

- $ (2x + 3)^2 $

$$
  (2x + 3)^2 = (2x + 3)(2x + 3) = 4x^2 + 12x + 9
$$

- $ (x + 2)^3 $

$$
  (x + 2)^3 = x^3 + 3x^2 \cdot 2 + 3x \cdot 2^2 + 2^3 = x^3 + 6x^2 + 12x + 8
$$

**4.**
> Factor each expression.

- $ 4x^2 - 25 $

$$
  4x^2 - 25 = (2x)^2 - 5^2 = (2x + 5)(2x - 5)
$$

- $ 2x^2 + 5x - 12 $

$$
  2x^2 + 5x - 12 = 2x^2 + 8x - 3x - 12 = 2x(x + 4) - 3(x + 4) = (2x - 3)(x + 4)
$$

- $ x^3 - 3x^2 - 4x + 12 $

- $ x^4 + 27x $

- $ 3x^{3/2} - 9x^{1/2} + 6x^{-1/2} $

- $ x^{3}y - 4xy $
